library/init/meta/tactic.lean
@@ -256,13 +256,13 @@ meta constant rename        : name → name → tactic unit
 meta constant clear         : expr → tactic unit
 meta constant revert_lst    : list expr → tactic nat
 meta constant whnf_core     : transparency → expr → tactic expr
-/- eta expand the given expression -/
+/- (head) eta expand the given expression -/
 meta constant eta_expand    : expr → tactic expr
-/- beta reduction -/
+/- (head) beta reduction -/
 meta constant beta          : expr → tactic expr
-/- zeta reduction -/
+/- (head) zeta reduction -/
 meta constant zeta          : expr → tactic expr
-/- eta reduction -/
+/- (head) eta reduction -/
 meta constant eta           : expr → tactic expr
 meta constant unify_core    : transparency → expr → expr → tactic unit
 /- is_def_eq_core is similar to unify_core, but it treats metavariables as constants. -/
