tests/lean/run/1331.lean
@@ -1,0 +1,24 @@
+def is_space : char → Prop
+| #" "    := true
+| #"\x09" := true -- \t
+| #"\n"   := true
+| #"\x0d" := true -- \r
+| _       := false
+
+instance is_space.decidable_pred : decidable_pred is_space :=
+begin delta is_space, apply_instance end
+
+def f (a : nat) : nat :=
+a + 2
+
+open tactic
+
+meta def check_target (p : pexpr) : tactic unit :=
+do t ← target, e ← to_expr p, guard (expr.alpha_eqv t e)
+
+lemma flemma : f 0 = 2 :=
+begin
+  delta f,
+  check_target `(0 + 2 = 2),
+  reflexivity
+end
